Unroll.v
@@ -1,35 +1,38 @@
 (* Implementation and correctness proofs for unrolled lists.
-   Andrew W. Appel, October 2010.  
+   Andrew W. Appel, October 2010.
 
  Required reading:
- Unrolling Lists, by Zhong Shao, John H. Reppy, and Andrew W. Appel. 
+ Unrolling Lists, by Zhong Shao, John H. Reppy, and Andrew W. Appel.
  Proc. 1994 ACM Conf. on Lisp and Functional Programming, June 1994.
  http://www.cs.princeton.edu/~appel/papers/unrolling-lists.pdf
 *)
 
 Require Import Permutation.
-Require Import SfLib. 
+Require Import SfLib.
 Definition admit {T: Type} : T.  Admitted.
 
 (** **** Exercise: 1 star (problem_1) *)
 (* Write a function [decreasing] such that it passes
   the following unit  tests (and similar ones for all numbers). *)
 
-Fixpoint decreasing {B} (f: nat -> B -> B) (base: B) (n: nat) : B := 
-  (* FILL IN HERE *) admit.
+Fixpoint decreasing {B} (f: nat -> B -> B) (base: B) (n: nat) : B :=
+  match n with
+    | O => base
+    | S n' => f n (decreasing f base n')
+  end.
 
 Example decreasing4: forall B (f: nat -> B -> B) x,
                decreasing f x 4 = f 4 (f 3 (f 2 (f 1 x))).
- (* FILL IN HERE *) Admitted.
+Proof. reflexivity. Qed.
 
 Example decreasing3: decreasing (@cons nat) nil 3 = 3::2::1::nil.
- (* FILL IN HERE *) Admitted.
+Proof. reflexivity. Qed.
 Example decreasing0:  forall B (f: nat->B->B) (x:B), decreasing f x 0 = x.
- (* FILL IN HERE *) Admitted.
+Proof. reflexivity. Qed.
 (** [] *)
 
 (** **** Exercise: 1 star (problem_2) *)
-(* The following function is in the Coq standard library.  
+(* The following function is in the Coq standard library.
  Fixpoint fold_right {A B: Type} (f: B -> A -> A) (a0: A) (l:list B) : A :=
     match l with
       | nil => a0
@@ -39,21 +42,27 @@ Example decreasing0:  forall B (f: nat->B->B) (x:B), decreasing f x 0 = x.
   Use fold_right to define a function to add up all the numbers in a list.
 *)
 
-Definition sum (l: list nat) : nat := 
- (* FILL IN HERE *) admit.
+Definition sum (l: list nat) : nat := fold_right plus 0 l.
 
-Lemma sum_decreasing: forall n, 
-             sum (decreasing (@cons _) nil n) = decreasing plus O n.
- (* FILL IN HERE *) Admitted.
+Lemma sum_decreasing: forall n,
+  sum (decreasing (@cons _) nil n) = decreasing plus O n.
+Proof.
+  intros. induction n; simpl. reflexivity. omega.
+Qed.
 (** [] *)
 
 (** **** Exercise: 2 stars (problem_3) *)
 (* Fun with permutations.  For useful lemmas, do "SearchAbout Permutation".  *)
 
-Lemma filter_permut:
-  forall (A: Type) (f: A -> bool) (l: list A),
-   Permutation (filter f l ++ filter (fun x => negb (f x)) l) l.
- (* FILL IN HERE *) Admitted.
+Lemma filter_permut: forall (A: Type) (f: A -> bool) (l: list A),
+  Permutation (filter f l ++ filter (fun x => negb (f x)) l) l.
+Proof.
+  intros. induction l; simpl.
+    reflexivity.
+    destruct (f a) eqn:Heqe; simpl.
+      constructor. assumption.
+      symmetry. apply Permutation_cons_app. symmetry. assumption.
+Qed.
 (** [] *)
 
 (* Best if viewed in Lucida Sans Unicode... *)
@@ -87,8 +96,8 @@ and a typical CPU can fetch the two "head" elements in a cell
 (such as 1,4   or 1,5)  in parallel.
 
 The representation of an unrolled list starts with a special
-"even" or "odd" cell, followed by a "tail" which is a chain of 
-two-head cons cells.  
+"even" or "odd" cell, followed by a "tail" which is a chain of
+two-head cons cells.
 
 However, the programmer wants to pretend that there is just
 an abstract data type (ADT) that behaves just like ordinary lists;
@@ -97,7 +106,7 @@ all the unrolling should be done "under the hood" by the compiler.
 In this exam you'll reason about this ADT using Coq.
 The goal is to have a set of types and functions as follows:
 
-  list' :    Type -> Type. 
+  list' :    Type -> Type.
   nil'  :    forall {X: Type}, list' X.
   cons':  forall {X: Type}, X -> list' X -> list' X.
   app':    forall {X: Type}, list' X -> list' X -> list' X.
@@ -106,47 +115,59 @@ and so on.
 *)
 
 (** **** Exercise: 2 stars (problem_4) *)
-(* Write inductive data type [tail] to represent the tail chain, 
+(* Write inductive data type [tail] to represent the tail chain,
   and the inductive data type [list']  to represent the even/odd header. *)
 
 Inductive tail (X: Type)  : Type :=
-(* FILL IN HERE *)
-.
+  | end' : tail X
+  | link' : X -> X -> tail X -> tail X.
 
 Inductive list' (X: Type) : Type :=
-(* FILL IN HERE *)
-.
+  | evenll : tail X -> list' X
+  | oddll : X -> tail X -> list' X.
 
-(* Use the Arguments command to make the X parameter of your 
+(* Use the Arguments command to make the X parameter of your
    data constructors implicit, as in the definition of "list" in Poly.v *)
-(* FILL IN HERE *)
+Arguments end' {X}.
+Arguments link' {X} _ _ _.
+Arguments evenll {X} _.
+Arguments oddll {X} _ _.
 (** [] *)
 
 (** **** Exercise: 2 stars (problem_5) *)
-(* Implement [nil'] that makes the empty [list'], and [cons'] that prepends one 
+(* Implement [nil'] that makes the empty [list'], and [cons'] that prepends one
   element.   To [cons'] a single element onto the front of an unrolled list, if the
   list was previously an even list it becomes an odd one, and vice versa. *)
 
-Definition nil' {X}:  list' X := 
- (* FILL IN HERE *) admit.
+Definition nil' {X}:  list' X := evenll end'.
 
 Definition cons' {X} (n: X) (l: list' X) : list' X :=
- (* FILL IN HERE *) admit.
+  match l with
+    | evenll xs => oddll n xs
+    | oddll x xs => evenll (link' n x xs)
+  end.
 (** [] *)
 
 (** **** Exercise: 2 stars (problem_6) *)
 (*  Write a function that converts a [list'] into an ordinary [list].
   Hint: write a helper function to walk down the tail. *)
 
-
+Fixpoint tail2list {X} (t: tail X) : list X :=
+  match t with
+    | end' => nil
+    | link' x y xs => x :: y :: tail2list xs
+  end.
 
 Definition list'2list {X} (l: list' X) : list X :=
- (* FILL IN HERE *) admit.
+  match l with
+    | evenll xs => tail2list xs
+    | oddll x xs => x :: tail2list xs
+  end.
 
 (*   The following unit test should work; if not, adjust your definitions. *)
 
 Example list'2list_12345: list'2list  (cons' 1 (cons' 2 (cons' 3 (cons' 4 (cons' 5 nil')))))  = [1;2;3;4;5].
- (* FILL IN HERE *) Admitted.
+Proof. reflexivity. Qed.
 (** [] *)
 
 (** **** Exercise: 1 star (list2list') *)
@@ -154,19 +175,44 @@ Example list'2list_12345: list'2list  (cons' 1 (cons' 2 (cons' 3 (cons' 4 (cons'
   list into an unrolled list. *)
 
 Definition list2list' {X} (l: list X) : list' X :=
- (* FILL IN HERE *) admit.
-
+  fold_right cons' nil' l.
 (** [] *)
 
 (** **** Exercise: 1 star *)
 (*  Prove that if you start with a list', convert it to a list, then convert back
     to a list', you get your original unrolled-list back.    *)
 
+Lemma cons_swap: forall X (l l': list' X) (x y : X),
+      cons' x (cons' y l) = cons' x (cons' y l')
+  -> cons' y (cons' x l) = cons' y (cons' x l').
+Proof.
+  intros. induction l; simpl; induction l'; inversion H; subst; reflexivity.
+Qed.
 
+Lemma cons_swap_odd: forall X (t t': tail X) (x y : X),
+     cons' x (oddll y t) = cons' x (oddll y t')
+  -> cons' y (oddll x t) = cons' y (oddll x t').
+Proof.
+  intros. induction t; simpl; induction t'; inversion H; subst; reflexivity.
+Qed.
 
-Lemma list'2list2list':
-  forall X (l: list' X), list2list' (list'2list l) = l.
-(* FILL IN HERE *) Admitted.
+Lemma cons_oddll_eq : forall X (t : tail X) (x : X),
+  cons' x (list2list' (tail2list t)) = oddll x t.
+Proof.
+  intros. induction t; simpl.
+    reflexivity.
+    destruct (list2list' (tail2list t)) eqn:Heqe; simpl.
+      simpl in IHt. inversion IHt. reflexivity.
+      inversion IHt.
+Qed.
+
+Lemma list'2list2list': forall X (l: list' X), list2list' (list'2list l) = l.
+Proof.
+  intros. destruct l; simpl.
+  - induction t; simpl. reflexivity.
+    rewrite IHt. reflexivity.
+  - apply cons_oddll_eq.
+Qed.
 (** [] *)
 
 (** **** Exercise: 2 stars *)
@@ -175,7 +221,12 @@ Lemma list'2list2list':
 
 Lemma list2list'2list:
   forall X (l: list X), list'2list (list2list' l) = l.
-(* FILL IN HERE *) Admitted.
+Proof.
+  intros. induction l; simpl.
+    reflexivity.
+    unfold list'2list. unfold cons'.
+    destruct (list2list' l); rewrite <- IHl; reflexivity.
+Qed.
 (** [] *)
 
 (** **** Exercise: 3 stars (fold_right') *)
@@ -187,21 +238,41 @@ Definition fold_right'_slow {A B: Type} (f: A-> B -> B) (base: B) (l: list' A) :
 
 (* This definition is correct, as it has the expected behavior: *)
 
-Lemma fold_right'_slow_example:  fold_right'_slow plus 0 (cons' 3 (cons' 5 nil')) = 8.
-(* FILL IN HERE *) Admitted.
+Lemma fold_right'_slow_example:
+  fold_right'_slow plus 0 (cons' 3 (cons' 5 nil')) = 8.
+Proof. reflexivity. Qed.
 
 (* The reason it's slow is that cons' keeps building and unbuilding the odd
-  and even list headers.  Define a more efficient fold_right' function that 
+  and even list headers.  Define a more efficient fold_right' function that
    just directly applies f (twice) for each (two-element) cell of the tail chain.
   As usual, you'll need an auxiliary function.  *)
 
-
+Fixpoint fold_right'tail {A B: Type} (f: A-> B -> B) (base: B) (l: tail A) : B :=
+  match l with
+    | end' => base
+    | link' x y xs => f x (f y (fold_right'tail f base xs))
+  end.
 
 Definition fold_right' {A B: Type} (f: A-> B -> B) (base: B) (l: list' A) : B :=
-(* FILL IN HERE *) admit.
+  match l with
+    | evenll xs => fold_right'tail f base xs
+    | oddll x xs => f x (fold_right'tail f base xs)
+  end.
+
+Lemma fold_right'tail_correct : forall A B (f: A -> B -> B) base t,
+  fold_right'tail f base t = fold_right f base (tail2list t).
+Proof.
+  intros. induction t; simpl.
+    reflexivity.
+    repeat f_equal. assumption.
+Qed.
 
 (* Now prove that you have the right function: *)
 Lemma fold_right'_correct:
   forall A B (f: A -> B -> B) base l, fold_right' f base l = fold_right'_slow f base l.
-(* FILL IN HERE *) Admitted.
+Proof.
+  intros. induction l; simpl;
+  unfold fold_right', fold_right'_slow; simpl;
+  repeat f_equal; apply fold_right'tail_correct.
+Qed.
 (** [] *)
