Redblack.v
@@ -1,25 +1,25 @@
 (* Implementation and proof of Red-Black Trees.  Andrew W. Appel, 2011 *)
 
 (* Required reading:
-Red-Black Trees in a Functional Setting, by Chris Okasaki. 
-Journal of Functional Programming, 9(4):471-477, July 1999. 
+Red-Black Trees in a Functional Setting, by Chris Okasaki.
+Journal of Functional Programming, 9(4):471-477, July 1999.
 http://www.eecs.usma.edu/webs/people/okasaki/jfp99redblack.pdf
 
    Optional reading:
-Efficient Verified Red-Black Trees, by Andrew W. Appel, September 2011. 
+Efficient Verified Red-Black Trees, by Andrew W. Appel, September 2011.
 http://www.cs.princeton.edu/~appel/papers/redblack.pdf
 *)
 
 (* Normally in Coq one might take the 2 Parameters and 3 Axioms and bundle
-   them into a Module Type ORDERED.  Then one would then express 
+   them into a Module Type ORDERED.  Then one would then express
    SET_OF_ORDERED as a parameterized module type (by ORDERED),
    and the module RedBlackTree as a functor (parameterized module).
-   This would be straightforward to do in Coq, but 
+   This would be straightforward to do in Coq, but
    is beyond the scope of this simple tutorial example.
 *)
 
 
-Ltac inv H := inversion H; clear H; subst. 
+Ltac inv H := inversion H; clear H; subst.
 
 Inductive order {key} (lt: key -> key -> Prop) (x y : key)  : Type :=
  Lt : lt x y -> order lt x y | Eq: x = y -> order lt x y | Gt: lt y x -> order lt x y.
@@ -60,13 +60,13 @@ Module Type SET_OF_ORDERED.
 
   Parameter interp: set -> (key -> Prop).
   Axiom interp_empty: forall x, ~ interp empty x.
-  Axiom interp_insert: 
-      forall x y s, 
-             valid s -> 
+  Axiom interp_insert:
+      forall x y s,
+             valid s ->
              ((x=y \/ interp s x) <-> interp (insert y s) x).
-  Axiom interp_member: 
-    forall x t, 
-      valid t -> 
+  Axiom interp_member:
+    forall x t,
+      valid t ->
       (member x t = true <-> interp t x).
 End SET_OF_ORDERED.
 
@@ -74,24 +74,24 @@ Module RedBlackTree: SET_OF_ORDERED.
 
  Inductive color := Red | Black.
  Inductive tree  : Type :=
- | E : tree 
+ | E : tree
  | T: color -> tree -> key -> tree -> tree.
 
  Fixpoint member (x: key) (t : tree) : bool :=
   match t with
   | E => false
-  | T _ tl k tr => if lt_dec x k then member x tl 
+  | T _ tl k tr => if lt_dec x k then member x tl
                          else if lt_dec k x then member x tr
                          else true
   end.
 
 Definition balance rb t1 k t2 :=
  match rb with Red => T Red t1 k t2
- | _ => 
- match t1 with 
+ | _ =>
+ match t1 with
  | T Red (T Red a x b) y c => T Red (T Black a x b) y (T Black c k t2)
  | T Red a x (T Red b y c) => T Red (T Black a x b) y (T Black c k t2)
- | a => match t2 with 
+ | a => match t2 with
             | T Red (T Red b y c) z d =>  T Red (T Black t1 k b) y (T Black c z d)
             | T Red b y (T Red c z d)  => T Red (T Black t1 k b) y (T Black c z d)
             | _ => T Black t1 k t2
@@ -99,14 +99,14 @@ Definition balance rb t1 k t2 :=
   end
  end.
 
-Definition makeBlack t := 
-  match t with 
+Definition makeBlack t :=
+  match t with
   | E => E
   | T _ a x b => T Black a x b
   end.
 
 Fixpoint ins x s :=
- match s with 
+ match s with
  | E => T Red E x E
  | T c a y b => if lt_dec x y then balance c (ins x a) y b
                         else if lt_dec y x then balance c a y (ins x b)
@@ -129,12 +129,12 @@ Lemma ins_not_E: forall x s, ins x s <> E.
 Proof.
 intros. induction s; simpl. intro Hx; inversion Hx.
 (* This one is best handled with a bit of proof automation,
-  but you can grind it out in a less automated way if you like 
+  but you can grind it out in a less automated way if you like
 *)
 (* FILL IN HERE *) Admitted.
 (** [] *)
 
-Definition ltopt (x y : option key) := 
+Definition ltopt (x y : option key) :=
   match x, y with
   | Some x', Some y' => lt x' y'
   | _, _ => True
@@ -151,22 +151,22 @@ Inductive searchtree: tree -> option key -> option key -> Prop :=
 
 (** **** Exercise: 3 stars (searchtree_balance) *)
 Lemma searchtree_balance:
- forall c  s1 t s2 lo hi, 
+ forall c  s1 t s2 lo hi,
    ltopt lo (Some t) -> ltopt (Some t) hi ->
    searchtree s1 lo (Some t) -> searchtree s2 (Some t) hi ->
     searchtree (balance c s1 t s2) lo hi.
 Proof.
 intros.
 unfold balance.
-(* This one is really painful to do without some proof automation. 
-  You can define a 12-line Ltac , "match goal with [7 clauses]", 
+(* This one is really painful to do without some proof automation.
+  You can define a 12-line Ltac , "match goal with [7 clauses]",
   and then simply repeat the application of that tactic. *)
 (* FILL IN HERE *) Admitted.
 (** [] *)
 
 (** **** Exercise: 2 stars (ins_is_searchtree) *)
-Lemma ins_is_searchtree: 
-   forall x s lo hi, ltopt lo (Some x) -> ltopt (Some x) hi -> 
+Lemma ins_is_searchtree:
+   forall x s lo hi, ltopt lo (Some x) -> ltopt (Some x) hi ->
                     searchtree s lo hi ->
                     searchtree (ins x s) lo hi.
 (* This one is pretty easy, even without proof automation *)
@@ -200,16 +200,16 @@ Lemma interp_empty: forall x, ~ interp' E x.
 (* FILL IN HERE *) Admitted.
 
 Lemma member_ok:
-  forall x t lo hi, 
-    searchtree t lo hi -> 
+  forall x t lo hi,
+    searchtree t lo hi ->
     if member x t then interp' t x else ~interp' t x.
 Proof.
 induction 1; intros.
 (* FILL IN HERE *) Admitted.
 
 Lemma interp_member:
-    forall x t, 
-      valid t -> 
+    forall x t,
+      valid t ->
       (member x t = true <-> interp' t x).
 (* FILL IN HERE *) Admitted.
 
@@ -228,17 +228,17 @@ Lemma interp'_balance:
 (** [] *)
 
 (** **** Exercise: 3 stars (ins_ok) *)
-Lemma ins_ok:  
-   forall x y t lo hi, 
-             searchtree t lo hi -> 
+Lemma ins_ok:
+   forall x y t lo hi,
+             searchtree t lo hi ->
              ((x=y \/ interp' t x) <-> interp' (ins y t) x).
 (* FILL IN HERE *) Admitted.
 (** [] *)
 
 (** **** Exercise: 3 stars (interp_insert) *)
 Lemma interp_insert:
-      forall x y s, 
-             valid s -> 
+      forall x y s,
+             valid s ->
              ((x=y \/ interp' s x) <-> interp' (insert y s) x).
 (* This one is easy, using previous lemmas ins_ok and interp'_makeBlack *)
 (* FILL IN HERE *) Admitted.
@@ -248,16 +248,16 @@ Lemma interp_insert:
   their functional specification for _correctness_, but does show that
   they will be _efficient_.  That is, one wants to know that the trees
    are balanced, i.e. that the deepest leaf is no more than twice as far
-   from the root as the shallowest leaf.  The predicate "is_redblack" 
+   from the root as the shallowest leaf.  The predicate "is_redblack"
    guarantees this; the lemma IsRB_leaf shows that the empty tree
   is balanced, and the lemma insert_is_redblack shows that balance
-  is preserved by insertion. 
+  is preserved by insertion.
 
   This is useful to prove, so we do it; but note that there's no way
-  of expressing such efficiency criteria in the specification, i.e. in the 
+  of expressing such efficiency criteria in the specification, i.e. in the
   Module Type SET_OF_ORDERED.
 *)
-  
+
 (** **** Exercise: 4 stars (is_redblack) *)
  Inductive is_redblack : tree -> color -> nat -> Prop :=
  | IsRB_leaf: forall c, is_redblack E c 0
@@ -276,14 +276,14 @@ Lemma is_redblack_toblack:
 Hint Resolve is_redblack_toblack.
 
 Lemma makeblack_fiddle:
-  forall s n, is_redblack s Black n -> 
+  forall s n, is_redblack s Black n ->
             exists n, is_redblack (makeBlack s) Red n.
 (* FILL IN HERE *) Admitted.
 
 Inductive nearly_redblack : tree -> nat -> Prop :=
  (* This predicate expresses, "the tree is a red-black tree, except that
-  it's nonempty and it is permitted to have two red nodes in a row at 
-  the very root (only)." 
+  it's nonempty and it is permitted to have two red nodes in a row at
+  the very root (only)."
 *)
 (* FILL IN HERE *)
  .
@@ -291,10 +291,10 @@ Inductive nearly_redblack : tree -> nat -> Prop :=
 (* FILL IN HERE *)
 
 Lemma ins_is_redblack:
-  forall x s n, 
+  forall x s n,
     (is_redblack s Black n -> nearly_redblack (ins x s) n) /\
     (is_redblack s Red n -> is_redblack (ins x s) Black n).
-(* This one is tedious with proof automation, 
+(* This one is tedious with proof automation,
    but extremely tedious without proof automation *)
 (* FILL IN HERE *) Admitted.
 
@@ -328,18 +328,9 @@ Extraction "redblack.ml" RedBlackTree.
   the range 0..N, then looking up N random keys in that range.
   With N = 1 million, the time on my desktop computer is about 1.5 seconds.
 
-  Usage:  
+  Usage:
    ocaml
    #use "redblack.ml";;
    #use "test_rb.ml";;
    test 1000000;;
  *)
-
-
-
-
-
-
-
-
-
